declarative typing goes through again

theories/DeclarativeTyping.v
@@ -1,130 +1,183 @@
 From MetaCoq.Template Require Import Universes.
-From MetaCoq.PCUIC Require Import PCUICAst.
-From LogRel Require Import Untyped Automation Notations.
+From MetaCoq.PCUIC Require Import PCUICAst PCUICRenameConv PCUICSigmaCalculus PCUICInstConv.
+From LogRel Require Import Untyped Notations GenericTyping Weakening.
 
 Set Primitive Projections.
 
-Inductive wfType  : context -> term -> Type :=
-    | wfTypeU {Γ} : 
-        [ |- Γ ] -> 
-        [ Γ |- U ] 
-    | wfTypeProd {Γ} {na : aname} {A B} : 
-        [ Γ |- A ] -> 
-        [Γ ,, (vass na A) |- B ] -> 
-        [ Γ |- tProd na A B ]
-    | wfTypeUniv {Γ} {A} :
-        [ Γ |- A : U ] -> 
-        [ Γ |- A ]
+Section Definitions.
 
-with wfContext : context -> Type :=
-    | connil : [ |- [] ]
-    | concons {Γ na A} : 
-        [ |- Γ ] -> 
-        [ Γ |- A ] -> 
-        [ |-  Γ ,, vass na A]
+  Inductive WfContextDecl : context -> Type :=
+      | connil : [ |- [] ]
+      | concons {Γ na A} : 
+          [ |- Γ ] -> 
+          [ Γ |- A ] -> 
+          [ |-  Γ ,, vass na A]
+  
+  with WfTypeDecl  : context -> term -> Type :=
+      | wfTypeU {Γ} : 
+          [ |- Γ ] -> 
+          [ Γ |- U ] 
+      | wfTypeProd {Γ} {na : aname} {A B} : 
+          [ Γ |- A ] -> 
+          [Γ ,, (vass na A) |- B ] -> 
+          [ Γ |- tProd na A B ]
+      | wfTypeUniv {Γ} {A} :
+          [ Γ |- A : U ] -> 
+          [ Γ |- A ]
 
-with wfTerm : context -> term -> term -> Type :=
-    | wfVar {Γ} {n decl} :
-        [   |- Γ ] ->
-        nth_error Γ n = Some decl ->
-        [ Γ |- tRel n : lift0 (S n) decl.(decl_type) ]
-    | wfTermProd {Γ} {na} {A B} :
-        [ Γ |- A : U] -> 
-        [Γ ,, (vass na A) |- B : U ] ->
-        [ Γ |- tProd na A B : U ]
-    | wfTermLam {Γ} {na} {A B t} :
-        [ Γ |- A ] ->        
-        [ Γ ,, vass na A |- t : B ] -> 
-        [ Γ |- tLambda na A t : tProd na A B]
-    | wfTermApp {Γ} {na} {f a A B} :
-        [ Γ |- f : tProd na A B ] -> 
-        [ Γ |- a : A ] -> 
-        [ Γ |- tApp f a : B{0 := a} ]
-    | wfTermConv {Γ} {t A B} :
-        [ Γ |- t : A ] -> 
-        [ Γ |- A ≅ B ] -> 
-        [ Γ |- t : B ]
-    
-with convType : context -> term -> term  -> Type :=  
-    | TypePiCong {Γ} {na nb} {A B C D} :
-        [ Γ |- A] ->
-        [ Γ |- A ≅ B] ->
-        [ Γ ,, vass na A |- C ≅ D] ->
-        [ Γ |- tProd na A C ≅ tProd nb B D]
-    | TypeRefl {Γ} {A} : 
-        [ Γ |- A ] -> 
-        [ Γ |- A ≅ A]       
-    | TypeSym {Γ} {A B} :
-        [ Γ |- A ≅ B ] -> 
-        [ Γ |- B ≅ A ]
-    | TypeTrans {Γ} {A B C} :
-        [ Γ |- A ≅ B] ->
-        [ Γ |- B ≅ C] ->
-        [ Γ |- A ≅ C]
-    | convUniv {Γ} {A B} :
-        [ Γ |- A ≅ B : U ] -> 
-        [ Γ |- A ≅ B ]    
+  with TypingDecl : context -> term -> term -> Type :=
+      | wfVar {Γ} {n decl} :
+          [   |- Γ ] ->
+          nth_error Γ n = Some decl ->
+          [ Γ |- tRel n : lift0 (S n) decl.(decl_type) ]
+      | wfTermProd {Γ} {na} {A B} :
+          [ Γ |- A : U] -> 
+          [Γ ,, (vass na A) |- B : U ] ->
+          [ Γ |- tProd na A B : U ]
+      | wfTermLam {Γ} {na} {A B t} :
+          [ Γ |- A ] ->        
+          [ Γ ,, vass na A |- t : B ] -> 
+          [ Γ |- tLambda na A t : tProd na A B]
+      | wfTermApp {Γ} {na} {f a A B} :
+          [ Γ |- f : tProd na A B ] -> 
+          [ Γ |- a : A ] -> 
+          [ Γ |- tApp f a : B{0 := a} ]
+      | wfTermConv {Γ} {t A B} :
+          [ Γ |- t : A ] -> 
+          [ Γ |- A ≅ B ] -> 
+          [ Γ |- t : B ]
+      
+  with ConvTypeDecl : context -> term -> term  -> Type :=  
+      | TypePiCong {Γ} {na nb} {A B C D} :
+          [ Γ |- A] ->
+          [ Γ |- A ≅ B] ->
+          [ Γ ,, vass na A |- C ≅ D] ->
+          [ Γ |- tProd na A C ≅ tProd nb B D]
+      | TypeRefl {Γ} {A} : 
+          [ Γ |- A ] -> 
+          [ Γ |- A ≅ A]       
+      | TypeSym {Γ} {A B} :
+          [ Γ |- A ≅ B ] -> 
+          [ Γ |- B ≅ A ]
+      | TypeTrans {Γ} {A B C} :
+          [ Γ |- A ≅ B] ->
+          [ Γ |- B ≅ C] ->
+          [ Γ |- A ≅ C]
+      | convUniv {Γ} {A B} :
+          [ Γ |- A ≅ B : U ] -> 
+          [ Γ |- A ≅ B ]    
 
-with convTerm : context -> term -> term -> term -> Type :=
-    | TermPiCong {Γ} {na nb } {A B C D} :
-        [ Γ |- A ] ->
-        [ Γ |- A ≅ B : U ] ->
-        [ Γ ,, vass na A |- C ≅ D : U ] ->
-        [ Γ |- tProd na A C ≅ tProd nb B D : U ]
-    | TermAppCong {Γ} {na} {a b f g A B} :
-        [ Γ |- f ≅ g : tProd na A B ] ->
-        [ Γ |- a ≅ b : A ] ->
-        [ Γ |- tApp f a ≅ tApp g b : B{0 := a} ]
-    | TermBRed {Γ} {na} {a t A B} :
-        [ Γ |- A ] ->
-        [ Γ ,, vass na A |- t : B ] ->
-        [ Γ |- a : A ] ->
-        [ Γ |- tApp (tLambda na A t) a ≅ t{0 := a} : B{0 := a} ]
-    | TermFunExt {Γ} {na nb} {f g A B} :
-        [ Γ |- A ] ->
-        [ Γ |- f : tProd na A B ] ->
-        [ Γ |- g : tProd nb A B ] ->
-        [ Γ ,, vass na A |- eta_expand f ≅ eta_expand g : B ] ->
-        [ Γ |- f ≅ g : tProd na A B ]
-    | TermRefl {Γ} {t A} :
-        [ Γ |- t : A ] -> 
-        [ Γ |- t ≅ t : A ]
-    | TermSym {Γ} {t t' A} :
-        [ Γ |- t ≅ t' : A ] ->
-        [ Γ |- t' ≅ t : A ]
-    | TermTrans {Γ} {t t' t'' A} :
-        [ Γ |- t ≅ t' : A ] ->
-        [ Γ |- t' ≅ t'' : A ] ->
-        [ Γ |- t ≅ t'' : A ]
-    | TermConv {Γ} {t t' A B} :
-        [ Γ |- t ≅ t': A ] ->
-        [ Γ |- A ≅ B ] ->
-        [ Γ |- t ≅ t': B ]
-    
-where "[   |- Γ ]" := (wfContext Γ)
-and   "[ Γ |- T ]" := (wfType Γ T)
-and   "[ Γ |- t : T ]" := (wfTerm Γ t T)
-and   "[ Γ |- A ≅ B ]" := (convType Γ A B)
-and   "[ Γ |- t ≅ t' : T ]" := (convTerm Γ t t' T).
+  with ConvTermDecl : context -> term -> term -> term -> Type :=
+      | TermPiCong {Γ} {na nb } {A B C D} :
+          [ Γ |- A ] ->
+          [ Γ |- A ≅ B : U ] ->
+          [ Γ ,, vass na A |- C ≅ D : U ] ->
+          [ Γ |- tProd na A C ≅ tProd nb B D : U ]
+      | TermAppCong {Γ} {na} {a b f g A B} :
+          [ Γ |- f ≅ g : tProd na A B ] ->
+          [ Γ |- a ≅ b : A ] ->
+          [ Γ |- tApp f a ≅ tApp g b : B{0 := a} ]
+      | TermBRed {Γ} {na} {a t A B} :
+          [ Γ |- A ] ->
+          [ Γ ,, vass na A |- t : B ] ->
+          [ Γ |- a : A ] ->
+          [ Γ |- tApp (tLambda na A t) a ≅ t{0 := a} : B{0 := a} ]
+      | TermFunExt {Γ} {na nb} {f g A B} :
+          [ Γ |- A ] ->
+          [ Γ |- f : tProd na A B ] ->
+          [ Γ |- g : tProd nb A B ] ->
+          [ Γ ,, vass na A |- eta_expand f ≅ eta_expand g : B ] ->
+          [ Γ |- f ≅ g : tProd na A B ]
+      | TermRefl {Γ} {t A} :
+          [ Γ |- t : A ] -> 
+          [ Γ |- t ≅ t : A ]
+      | TermSym {Γ} {t t' A} :
+          [ Γ |- t ≅ t' : A ] ->
+          [ Γ |- t' ≅ t : A ]
+      | TermTrans {Γ} {t t' t'' A} :
+          [ Γ |- t ≅ t' : A ] ->
+          [ Γ |- t' ≅ t'' : A ] ->
+          [ Γ |- t ≅ t'' : A ]
+      | TermConv {Γ} {t t' A B} :
+          [ Γ |- t ≅ t': A ] ->
+          [ Γ |- A ≅ B ] ->
+          [ Γ |- t ≅ t': B ]
+      
+  where "[   |- Γ ]" := (WfContextDecl Γ)
+  and   "[ Γ |- T ]" := (WfTypeDecl Γ T)
+  and   "[ Γ |- t : T ]" := (TypingDecl Γ t T)
+  and   "[ Γ |- A ≅ B ]" := (ConvTypeDecl Γ A B)
+  and   "[ Γ |- t ≅ t' : T ]" := (ConvTermDecl Γ t t' T).
+
+  Inductive OneRedTermDecl (Γ : context) : term -> term -> term -> Type :=
+  | appSubst {na A B t u a} :
+      [ Γ |- t ⇒ u : tProd na A B] ->
+      [ Γ |- a : A ] ->
+      [ Γ |- tApp t a ⇒ tApp u a : B{0 := a} ]
+  | BRed {na} {A B a t} :
+      [ Γ |- A ] -> 
+      [ Γ ,, vass na A |- t : B ] ->
+      [ Γ |- a : A ] ->
+      [ Γ |- tApp (tLambda na A t) a ⇒ t{0 := a} : B{0 := a} ]
+  | termRedConv {A B t u} : 
+      [ Γ |- t ⇒ u : A ] ->
+      [ Γ |- A ≅ B ] ->
+      [ Γ |- t ⇒ u : B ]
+
+  where "[ Γ |- t ⇒ u : A ]" := (OneRedTermDecl Γ t u A).
+
+  Inductive OneRedTypeDecl (Γ : context) : term -> term -> Type :=
+  | typeRedUniv {A B} :
+      [ Γ |- A ⇒ B : U ] ->
+      [ Γ |- A ⇒ B ]
+
+  where "[ Γ |- A ⇒ B ]" := (OneRedTypeDecl Γ A B).
+
+End Definitions.
+
+Module DeclarativeTypingData.
+
+  #[export] Instance WfContext_Decl : WfContext de := WfContextDecl.
+  #[export] Instance WfType_Decl : WfType de := WfTypeDecl.
+  #[export] Instance Typing_Decl : Typing de := TypingDecl.
+  #[export] Instance ConvType_Decl : ConvType de := ConvTypeDecl.
+  #[export] Instance ConvTerm_Decl : ConvTerm de := ConvTermDecl.
+  #[export] Instance ConvNeu_Decl : ConvNeu de := ConvTermDecl.
+  #[export] Instance OneRedType_Decl : OneRedType de := OneRedTypeDecl.
+  #[export] Instance OneRedTerm_Decl : OneRedTerm de := OneRedTermDecl.
+  #[export, refine] Instance DeclTypingData : GenericTypingData de := {}.
+  Defined.
+
+  Ltac fold_decl :=
+    change WfContextDecl with wf_context in * ;
+    change WfTypeDecl with wf_type in *;
+    change TypingDecl with typing in * ;
+    change ConvTypeDecl with conv_type in * ;
+    change ConvTermDecl with conv_term in * ;
+    change OneRedTypeDecl with red_ty in *;
+    change OneRedTermDecl with red_tm in *.
+
+End DeclarativeTypingData.
 
 Section InductionPrinciples.
-
+  Open Scope untagged_scope.
+  Import DeclarativeTypingData.
 
 Scheme 
-    Minimality for wfContext Sort Type with
-    Minimality for wfType    Sort Type with
-    Minimality for wfTerm    Sort Type with
-    Minimality for convType  Sort Type with
-    Minimality for convTerm  Sort Type.
+    Minimality for WfContextDecl Sort Type with
+    Minimality for WfTypeDecl   Sort Type with
+    Minimality for TypingDecl    Sort Type with
+    Minimality for ConvTypeDecl  Sort Type with
+    Minimality for ConvTermDecl  Sort Type.
 
-Combined Scheme wfInduction from
-    wfContext_rect_nodep,
-    wfType_rect_nodep,
-    wfTerm_rect_nodep,
-    convType_rect_nodep,
-    convTerm_rect_nodep.
+Combined Scheme _WfDeclInduction from
+    WfContextDecl_rect_nodep,
+    WfTypeDecl_rect_nodep,
+    TypingDecl_rect_nodep,
+    ConvTypeDecl_rect_nodep,
+    ConvTermDecl_rect_nodep.
 
-Definition wfInductionType
+Definition WfDeclInductionConcl
   (PCon : context -> Type) (PTy : context -> term -> Type)
   (PTm PTyEq : context -> term -> term -> Type)
   (PTmEq : context -> term -> term -> term -> Type) :=
@@ -134,253 +187,205 @@ Definition wfInductionType
 	× (forall (Γ : context) (A B : term), [Γ |- A ≅ B] -> PTyEq Γ A B)
   × (forall (Γ : context) (t u A : term), [Γ |- t ≅ u : A] -> PTmEq Γ t u A).
 
+Let WfDeclInductionType := ltac:
+  (
+  set (H := _WfDeclInduction) ;
+  fold_decl ;
+  let ty := type of H in exact ty).
+
+Definition WfDeclInduction : WfDeclInductionType := _WfDeclInduction.
 
 End InductionPrinciples.
 
-Lemma termMetaConv (Γ : context) (t A B : term) :
-  [Γ |- t : A] ->
-  A = B ->
-  [Γ |- t : B].
-Proof.
-  now intros ? ->.
-Qed.
-
-Lemma eqTermMetaConv (Γ : context) (t u A B : term) :
-  [Γ |- t ≅ u : A] ->
-  A = B ->
-  [Γ |- t ≅ u : B].
-Proof.
-  now intros ? ->.
-Qed.
-
-Inductive termRed (Γ : context) : term -> term -> term -> Type :=
-    | appSubst {na A B t u a} :
-        [ Γ |- t ⇒ u : tProd na A B] ->
-        [ Γ |- a : A ] ->
-        [ Γ |- tApp t a ⇒ tApp u a : B{0 := a} ]
-    | BRed {na} {A B a t} :
-        [ Γ |- A ] -> 
-        [ Γ ,, vass na A |- t : B ] ->
-        [ Γ |- a : A ] ->
-        [ Γ |- tApp (tLambda na A t) a ⇒ t{0 := a} : B{0 := a} ]
-    | termRedConv {A B t u} : 
-        [ Γ |- t ⇒ u : A ] ->
-        [ Γ |- A ≅ B ] ->
-        [ Γ |- t ⇒ u : B ]
-
-where "[ Γ |- t ⇒ u : A ]" := (termRed Γ t u A).
-
-Inductive typeRed (Γ : context) : term -> term -> Type :=
-    | typeRedUniv {A B} :
-        [ Γ |- A ⇒ B : U ] ->
-        [ Γ |- A ⇒ B ]
-
-where "[ Γ |- A ⇒ B ]" := (typeRed Γ A B).
-
-#[global] Hint Constructors wfType wfContext wfTerm convType convTerm : mltt.
-#[global] Hint Constructors termRed typeRed termRedClosure typeRedClosure
-  termRedWHNF typeRedWHNF termEqWF typeEqWF termRedWF typeRedWF : mltt.
-
-(*Making the non syntax-directed hints more costly*)
-#[global] Remove Hints wfTermConv TermConv termRedConv TypeTrans TermTrans
-  termRedSucc typeRedSucc : mltt.
-#[global] Hint Resolve wfTermConv TermConv termRedConv TypeTrans TermTrans
-  termRedSucc typeRedSucc | 6 : mltt.
-
-#[global] Hint Resolve termRedWHNFRed termRedWHNFWHNF typeRedWHNFRed typeRedWHNFWHNF 
-  termEqWFLeft termEqWFRight termEqWFEq typeEqWFLeft typeEqWFRight typeEqWFEq
-  termRedWFLeft termRedWFRight termRedWFRed typeRedWFLeft typeRedWFRight
-  typeRedWFRed : mltt.
-
-
 Section TypingWk.
+  Open Scope untagged_scope.
+  Import DeclarativeTypingData.
 
-Variable foo : context_decl.
-
-Lemma nth_error_wk (Γ Δ : context) n decl (ρ : Δ ≤ Γ) :
-  nth_error Γ n = Some decl ->
-  {decl' & nth_error Δ (ρ n) = Some decl' ×
-    map_decl (rename (ρ ∘ rshiftk (S n))) decl = map_decl (rename (rshiftk (S (ρ n)))) decl'}.
-Proof.
-  intros Hdecl.
-  destruct ρ as [ρ wfρ] ; cbn.
-  induction wfρ in n, Hdecl |- *.
-  - exists decl.
-    split.
-    1: easy.
-    reflexivity.
-  - cbn.
-    edestruct IHwfρ as [decl' [? IH]].
-    1: eassumption.
-    eexists ; split.
-    1: eassumption.
-    now rewrite <- rename_compose, <- compose_map_decl, IH, compose_map_decl, rename_compose.
-  - destruct n as [ | n].
-    + cbn in *.
-      inversion Hdecl ; subst ; clear Hdecl.
-      eexists ; split.
-      1: reflexivity.
-      unfold map_decl ; cbn.
-      f_equal.
-      rewrite <- rename_inst, rename_compose.
-      apply rename_ext.
-      intros ?.
-      now rewrite Nat.sub_0_r.
-    + cbn in *.
+  Lemma nth_error_wk (Γ Δ : context) n decl (ρ : Δ ≤ Γ) :
+    nth_error Γ n = Some decl ->
+    {decl' & nth_error Δ (ρ n) = Some decl' ×
+      map_decl (rename (ρ ∘ rshiftk (S n))) decl = map_decl (rename (rshiftk (S (ρ n)))) decl'}.
+  Proof.
+    intros Hdecl.
+    destruct ρ as [ρ wfρ] ; cbn.
+    induction wfρ in n, Hdecl |- *.
+    - exists decl.
+      split.
+      1: easy.
+      reflexivity.
+    - cbn.
       edestruct IHwfρ as [decl' [? IH]].
       1: eassumption.
       eexists ; split.
-      1: now rewrite Nat.sub_0_r.
-      now rewrite <- rename_compose, <- compose_map_decl, IH, compose_map_decl, rename_compose, Nat.sub_0_r.
-  Qed.
+      1: eassumption.
+      now rewrite <- rename_compose, <- compose_map_decl, IH, compose_map_decl, rename_compose.
+    - destruct n as [ | n].
+      + cbn in *.
+        inversion Hdecl ; subst ; clear Hdecl.
+        eexists ; split.
+        1: reflexivity.
+        unfold map_decl ; cbn.
+        f_equal.
+        rewrite <- rename_inst, rename_compose.
+        apply rename_ext.
+        intros ?.
+        now rewrite Nat.sub_0_r.
+      + cbn in *.
+        edestruct IHwfρ as [decl' [? IH]].
+        1: eassumption.
+        eexists ; split.
+        1: now rewrite Nat.sub_0_r.
+        now rewrite <- rename_compose, <- compose_map_decl, IH, compose_map_decl, rename_compose, Nat.sub_0_r.
+    Qed.
 
-Let PCon (Γ : context) := True.
-Let PTy (Γ : context) (A : term) := forall Δ (ρ : Δ ≤ Γ), [|- Δ ] -> [Δ |- A.[ren ρ]].
-Let PTm (Γ : context) (t A : term) := forall Δ (ρ : Δ ≤ Γ), [|- Δ ] ->
-  [Δ |- t.[ren ρ] : A.[ren ρ]].
-Let PTyEq (Γ : context) (A B : term) := forall Δ (ρ : Δ ≤ Γ), [|- Δ ] ->
-  [Δ |- A.[ren ρ] ≅ B.[ren ρ]].
-Let PTmEq (Γ : context) (t u A : term) := forall Δ (ρ : Δ ≤ Γ), [|- Δ ] ->
-  [Δ |- t.[ren ρ] ≅ u.[ren ρ] : A.[ren ρ]].
+  Let PCon (Γ : context) := True.
+  Let PTy (Γ : context) (A : term) := forall Δ (ρ : Δ ≤ Γ), [|- Δ ] -> [Δ |- A.[ren ρ]].
+  Let PTm (Γ : context) (t A : term) := forall Δ (ρ : Δ ≤ Γ), [|- Δ ] ->
+    [Δ |- t.[ren ρ] : A.[ren ρ]].
+  Let PTyEq (Γ : context) (A B : term) := forall Δ (ρ : Δ ≤ Γ), [|- Δ ] ->
+    [Δ |- A.[ren ρ] ≅ B.[ren ρ]].
+  Let PTmEq (Γ : context) (t u A : term) := forall Δ (ρ : Δ ≤ Γ), [|- Δ ] ->
+    [Δ |- t.[ren ρ] ≅ u.[ren ρ] : A.[ren ρ]].
 
-
-Theorem typing_wk : wfInductionType PCon PTy PTm PTyEq PTmEq.
-Proof.
-  apply wfInduction.
-  - red.
-    trivial.
-  - red. trivial.
-  - intros ? ? IH.
-    now econstructor.
-  - intros Γ na A B HA IHA HB IHB Δ ρ HΔ.
-    econstructor ; fold inst.
-    1: easy.
-    replace (B.[up 1 (ren ρ)]) with (B.[ren (wk_lift ρ)])
-      by now rewrite ren_shiftn.
-    unshelve eapply (IHB _ {| wk := wk_lift ρ ; well_wk := _ |} _).
-    all: now econstructor.
-  - intros * _ IHA ? * ?.
-    econstructor.
-    now eapply IHA.
-  - intros * _ IHΓ Hnth ? * ?.
-    unshelve eapply nth_error_wk in Hnth as [decl' [? edecl]] ; tea.
-    unfold ren at 1.
-    cbn.
-    eapply termMetaConv.
-    1: econstructor ; eassumption.
-    rewrite <- rename_inst, ! lift_rename, rename_compose, (map_decl_type _ decl'), (map_decl_type _ decl).
-    f_equal.
-    rewrite ! lift_renaming_0_rshift, <- edecl.
-    eapply map_decl_ext ; intros ; eapply rename_ext ; intros ?.
-    now rewrite lift_renaming_0_rshift.
-  - intros * _ IHA _ IHB ? ρ ?.
-    cbn.
-    econstructor.
-    1: now eapply IHA.
-    replace B.[_] with B.[ren (wk_lift ρ)] by now rewrite ren_shiftn.
-    unshelve eapply (IHB _ {| wk := wk_lift ρ ; well_wk := _ |} _).
-    1: now econstructor.
-    econstructor ; tea.
-    econstructor.
-    now eapply IHA.
-  - intros * _ IHA _ IHt ? ρ ?.
-    cbn.
-    econstructor.
-    1: now eapply IHA.
-    red in IHt.
-    replace t.[_] with t.[ren (wk_lift ρ)] by now rewrite ren_shiftn.
-    replace B.[_] with B.[ren (wk_lift ρ)] by now rewrite ren_shiftn.
-    unshelve eapply (IHt _ {| wk := wk_lift ρ ; well_wk := _ |} _).
-    1: now econstructor.
-    econstructor ; tea.
-    now eapply IHA.
-  - intros * _ IHf _ IHu ? ρ ?.
-    cbn.
-    rewrite subst10_inst.
-    replace B.[_] with B.[(up 1 (ren ρ))] by (now rewrite up_Up).
-    econstructor.
-    2: now eapply IHu.
-    now eapply IHf.
-  - intros * _ IHt _ IHAB ? ρ ?.
-    econstructor.
-    1: now eapply IHt.
-    now eapply IHAB.
-  - intros Γ ? ? A A' B B' _ IHA _ IHAA' _ IHBB' ? ρ ?.
-    cbn.
-    econstructor.
-    + now eapply IHA.
-    + now eapply IHAA'.
-    + replace B.[_] with B.[ren (wk_lift ρ)] by now rewrite ren_shiftn.
-      replace B'.[_] with B'.[ren (wk_lift ρ)] by now rewrite ren_shiftn.
-      unshelve eapply (IHBB' _ {| wk := wk_lift ρ ; well_wk := _ |} _).
+  Theorem typing_wk : WfDeclInductionConcl PCon PTy PTm PTyEq PTmEq.
+  Proof.
+    apply WfDeclInduction.
+    - red.
+      trivial.
+    - red. trivial.
+    - intros ? ? IH.
+      now econstructor.
+    - intros Γ na A B HA IHA HB IHB Δ ρ HΔ.
+      econstructor ; fold inst.
+      1: now eapply IHA.
+      replace (B.[up 1 (ren ρ)]) with (B.[ren (wk_lift ρ)])
+        by now rewrite ren_shiftn.
+      unshelve eapply (IHB _ {| wk := wk_lift ρ ; well_wk := _ |} _).
+      1: now constructor.
+      now constructor ; fold_decl.
+    - intros * _ IHA ? * ?.
+      econstructor.
+      now eapply IHA.
+    - intros * _ IHΓ Hnth ? * ?.
+      unshelve eapply nth_error_wk in Hnth as [decl' [? edecl]] ; tea.
+      unfold ren at 1.
+      cbn.
+      eapply typing_meta_conv.
+      1: econstructor ; eassumption.
+      rewrite <- rename_inst, ! lift_rename, rename_compose, (map_decl_type _ decl'), (map_decl_type _ decl).
+      f_equal.
+      setoid_rewrite lift_renaming_0_rshift.
+      rewrite <- edecl.
+      eapply map_decl_ext ; intros ; eapply rename_ext ; intros ?.
+      now rewrite lift_renaming_0_rshift.
+    - intros * _ IHA _ IHB ? ρ ?.
+      cbn.
+      econstructor.
+      1: now eapply IHA.
+      replace B.[_] with B.[ren (wk_lift ρ)] by now rewrite ren_shiftn.
+      unshelve eapply (IHB _ {| wk := wk_lift ρ ; well_wk := _ |} _).
+      1: now econstructor.
+      econstructor ; tea.
+      econstructor.
+      now eapply IHA.
+    - intros * _ IHA _ IHt ? ρ ?.
+      cbn.
+      econstructor.
+      1: now eapply IHA.
+      red in IHt.
+      replace t.[_] with t.[ren (wk_lift ρ)] by now rewrite ren_shiftn.
+      replace B.[_] with B.[ren (wk_lift ρ)] by now rewrite ren_shiftn.
+      unshelve eapply (IHt _ {| wk := wk_lift ρ ; well_wk := _ |} _).
       1: now econstructor.
       econstructor ; tea.
       now eapply IHA.
-  - intros * _ IHA ? ρ ?.
-    eapply TypeRefl.
-    now eapply IHA.
-  - intros * _ IH ? ρ ?.
-    econstructor.
-    now eapply IH.
-  - intros * _ IHA _ IHB ? ρ ?.
-    eapply TypeTrans.
-    + now eapply IHA.
-    + now eapply IHB.
-  - intros * _ IH ? ρ ?.
-    eapply convUniv.
-    now eapply IH.
-  - intros Γ ? ? A A' B B' _ IHA _ IHAA' _ IHBB' ? ρ ?.
-    cbn.
-    econstructor.
-    + now eapply IHA.
-    + now eapply IHAA'.
-    + replace B.[_] with B.[ren (wk_lift ρ)] by now rewrite ren_shiftn.
-      replace B'.[_] with B'.[ren (wk_lift ρ)] by now rewrite ren_shiftn.
-      unshelve eapply (IHBB' _ {| wk := wk_lift ρ ; well_wk := _ |} _).
-      all: now econstructor.
-  - intros Γ ? u u' f f' A B _ IHf _ IHu ? ρ ?.
-    cbn.
-    rewrite subst10_inst.
-    replace B.[_] with B.[(up 1 (ren ρ))] by (now rewrite up_Up).
-    now econstructor.
-  - intros Γ ? u t A B _ IHA _ IHt _ IHu ? ρ ?.
-    cbn. 
-    rewrite ! subst10_inst.
-    replace t.[⇑ _] with t.[(up 1 (ren ρ))] by (now rewrite up_Up).
-    replace t.[_] with t.[ren (wk_lift ρ)] by (now rewrite ren_shiftn).
-    replace B.[_] with B.[ren (wk_lift ρ)] by (now rewrite <- up_Up, ren_shiftn).
-    econstructor.
-    1,3: easy.
-    unshelve eapply (IHt _ {| wk := wk_lift ρ ; well_wk := _ |} _).
-    all: now econstructor.
-  - intros Γ ? ? f f' A B _ IHA _ IHf _ IHg _ IHe ? ρ ?.
-    cbn.
-    econstructor.
-    1-3: easy.
-    unshelve epose proof (IHe _ {| wk := wk_lift ρ ; well_wk := _ |} _) as IHe'.
-    2: now econstructor.
-    1: now econstructor.
-    cbn in *.
-    unfold ren in IHe' at 3 5.
-    unfold eta_expand.
-    cbn in *.
-    rewrite ! lift0_inst, ! inst_assoc in IHe' |- *.
-    replace B.[_] with B.[ren (shiftn 1 ρ)] by (now rewrite ren_shiftn).
-    unshelve erewrite (inst_ext _ _ _ f), (inst_ext _ _ _ f').
-    5: eassumption.
-    all: rewrite <- Upn_ren.
-    all: change 1 with (0 + 1).
-    all: rewrite <- subst_shift_comm.
-    all: cbn.
-    all: now rewrite Upn_0.
-  - intros * _ IHt ? ρ ?.
-    now econstructor.
-  - intros * _ IHt ? ρ ?.
-    now econstructor.
-  - intros * _ IHt _ IHt' ? ρ ?.
-    now eapply TermTrans.
-  - intros * _ IHt _ IHA ? ρ ?.
-    now eapply TermConv.
-Qed.
+    - intros * _ IHf _ IHu ? ρ ?.
+      cbn.
+      rewrite subst10_inst.
+      replace B.[_] with B.[(up 1 (ren ρ))] by (now rewrite up_Up).
+      econstructor.
+      2: now eapply IHu.
+      now eapply IHf.
+    - intros * _ IHt _ IHAB ? ρ ?.
+      econstructor.
+      1: now eapply IHt.
+      now eapply IHAB.
+    - intros Γ ? ? A A' B B' _ IHA _ IHAA' _ IHBB' ? ρ ?.
+      cbn.
+      econstructor.
+      + now eapply IHA.
+      + now eapply IHAA'.
+      + replace B.[_] with B.[ren (wk_lift ρ)] by now rewrite ren_shiftn.
+        replace B'.[_] with B'.[ren (wk_lift ρ)] by now rewrite ren_shiftn.
+        unshelve eapply (IHBB' _ {| wk := wk_lift ρ ; well_wk := _ |} _).
+        1: now econstructor.
+        econstructor ; tea.
+        now eapply IHA.
+    - intros * _ IHA ? ρ ?.
+      eapply TypeRefl.
+      now eapply IHA.
+    - intros * _ IH ? ρ ?.
+      econstructor.
+      now eapply IH.
+    - intros * _ IHA _ IHB ? ρ ?.
+      eapply TypeTrans.
+      + now eapply IHA.
+      + now eapply IHB.
+    - intros * _ IH ? ρ ?.
+      eapply convUniv.
+      now eapply IH.
+    - intros Γ ? ? A A' B B' _ IHA _ IHAA' _ IHBB' ? ρ ?.
+      cbn.
+      econstructor.
+      + now eapply IHA.
+      + now eapply IHAA'.
+      + replace B.[_] with B.[ren (wk_lift ρ)] by now rewrite ren_shiftn.
+        replace B'.[_] with B'.[ren (wk_lift ρ)] by now rewrite ren_shiftn.
+        unshelve eapply (IHBB' _ {| wk := wk_lift ρ ; well_wk := _ |} _).
+        1: now econstructor.
+        all: now econstructor ; fold_decl.
+    - intros Γ ? u u' f f' A B _ IHf _ IHu ? ρ ?.
+      cbn.
+      rewrite subst10_inst.
+      replace B.[_] with B.[(up 1 (ren ρ))] by (now rewrite up_Up).
+      now econstructor ; fold_decl.
+    - intros Γ ? u t A B _ IHA _ IHt _ IHu ? ρ ?.
+      cbn. 
+      rewrite ! subst10_inst.
+      replace t.[⇑ _] with t.[(up 1 (ren ρ))] by (now rewrite up_Up).
+      replace t.[_] with t.[ren (wk_lift ρ)] by (now rewrite ren_shiftn).
+      replace B.[_] with B.[ren (wk_lift ρ)] by (now rewrite <- up_Up, ren_shiftn).
+      econstructor ; fold_decl.
+      1,3: easy.
+      unshelve eapply (IHt _ {| wk := wk_lift ρ ; well_wk := _ |} _).
+      all: now econstructor ; fold_decl.
+    - intros Γ ? ? f f' A B _ IHA _ IHf _ IHg _ IHe ? ρ ?.
+      cbn.
+      econstructor ; fold_decl.
+      1-3: easy.
+      unshelve epose proof (IHe _ {| wk := wk_lift ρ ; well_wk := _ |} _) as IHe'.
+      2: now econstructor.
+      1: now econstructor ; fold_decl.
+      cbn in *.
+      unfold ren in IHe' at 3 5.
+      cbn in *.
+      rewrite ! lift0_inst, ! inst_assoc in IHe' |- *.
+      replace B.[_] with B.[ren (shiftn 1 ρ)] by (now rewrite ren_shiftn).
+      unshelve erewrite (inst_ext _ _ _ f), (inst_ext _ _ _ f').
+      5: eassumption.
+      all: rewrite <- Upn_ren.
+      all: change 1 with (0 + 1).
+      all: rewrite <- subst_shift_comm.
+      all: cbn.
+      all: now rewrite Upn_0.
+    - intros * _ IHt ? ρ ?.
+      now econstructor ; fold_decl.
+    - intros * _ IHt ? ρ ?.
+      now econstructor ; fold_decl.
+    - intros * _ IHt _ IHt' ? ρ ?.
+      now eapply TermTrans ; fold_decl.
+    - intros * _ IHt _ IHA ? ρ ?.
+      now eapply TermConv ; fold_decl.
+  Qed.
 
 End TypingWk.
